Makefile
@@ -41,6 +41,7 @@ SPEC_FILES = \
 IMPL_FILES = \
   src/impl/TLS13.LowTypes.fsti \
   src/impl/TLS13.Extract.Smoke.fst \
+  src/impl/TLS13.State.fst \
   src/impl/TLS13.Crypto.fsti \
   src/impl/TLS13.KeySchedule.fsti \
   src/impl/TLS13.X509.fsti \
